\subsection{\texttt{El} equations for the Mahlo canonicity model}

Here we prove that the El predicate for the Mahlo universe respects the equations of El of Mahlo in syntax.

\begin{verbatim}
ElEl0ᴾ : (γ : Sub · Γ) (γᴾ : Γᴾ γ) → (u : Tm Γ U0)
            → (el0 : Tm Γ (El0 $ u)) →
  (El El0 U+ El+ $$ (El0' u))ᴾ γ γᴾ el0[γ]
  ≡
  (El0 u)ᴾ γ γᴾ el0[γ]

  Elᴾ ... El0[γ] (El0ᴾ γ γᴾ) ... (El0' u[γ]) ((El0' u)ᴾ γ γᴾ) el0[γ]
  ≡
  (El0 u)ᴾ γ γᴾ el0[γ]

  El0ᴾ γ γᴾ u[γ] (uᴾ γ γᴾ) el0[γ]
  ≡
  El0ᴾ γ γᴾ u[γ] (uᴾ γ γᴾ) el0[γ]

ElEl+ᴾ : (γ : Sub · Γ) (γᴾ : Γᴾ γ) → (A : Tm ∙ Ma)
          → (B : Tm ∙ El A → Ma)
          → (C : Tm ∙ (U+ $$ (El A) $$
                             (lam (El[p] $$ (B[p] $$ q)))))
          → (el+ : Tm Γ (El {U+} {El+} (El+ $$ C))) →
  (El {U+} {El+} $$ (El+ A B C))ᴾ  γ γᴾ el+[γ]
  ≡
  (El+ (El $$ A) (lam (El[p] $$ B[p] $$ q)) (El C))ᴾ γ γᴾ el+[γ]

  El+ᴾ (El $$ A[γ]) (Elᴾ A[γ] (Aᴾ γ γᴾ))
     ((lam (El[p] $$ (B[p] $$ q)))[γ])
     (λ a aᴾ → Elᴾ ((B $$ a)[γ]) (Bᴾ γ γᴾ a aᴾ))
     C[γ] (Cᴾ γ γᴾ) el+[γ]
  ≡
  El+ᴾ (El $$ A[γ]) (Elᴾ A[γ] (Aᴾ γ γᴾ))
                  ((lam (El[p] $$ (B[p] $$ q)))[γ])
      (λ a aᴾ → Elᴾ ((app B)[γ,a]) (Bᴾ γ γᴾ a aᴾ))
      C[γ] (Cᴾ γ γᴾ) el+[γ]
\end{verbatim}

\subsection{\texttt{maElim} equations for the Mahlo canonicity model}

Checking that the $\beta$ rules for eliminator of \texttt{Ma} are respected by the canonicity model.

\begin{verbatim}
El0maElimᴾ : (γ : Sub · Γ) (γᴾ : Γᴾ γ) →
        {j : MetaNat}(P : Tm Γ (Ma → (U j))
        → (el0 : Tm Γ (U0 → P $$ (El0' $$ q)))
        → (el+ : Tm Γ (Ma → P $$ q → (El $$ q¹ → Ma)
          → (lam (P[p] $$ (q¹ $$ q)))
          → U+ $$ (El $$ q³) $$ lam (El[p] $$ (q² $$ q))
          → P $$ (El+' $$ q⁴ $$ q² $$ q))) →
        (x : Tm Γ U0) →
  (maElim P el0 el+ (El0' x))ᴾ γ γᴾ
  ≡
  (el0 x)ᴾ γ γᴾ

  MaᴾElim P[γ] (Pᴾ γ γᴾ)
      el0[γ] (λ u uᴾ → el0ᴾ γ γᴾ u uᴾ) el+[γ]
      (λ A Aᴾ PA PAᴾ B Bᴾ PB PBᴾ C Cᴾ →
        el+ᴾ γ γᴾ A Aᴾ PA PAᴾ B Bᴾ PB PBᴾ C Cᴾ)
      (El0' x[γ]) (El0'ᴾ x[γ] (xᴾ γ γᴾ))
  ≡
  el0ᴾ γ γᴾ x[γ] (xᴾ γ γᴾ)

  (λ u uᴾ → el0ᴾ γ γᴾ u uᴾ) x[γ] (xᴾ γ γᴾ)
  ≡
  el0ᴾ γ γᴾ x[γ] (xᴾ γ γᴾ)

  el0ᴾ γ γᴾ x[γ] (xᴾ γ γᴾ)
  ≡
  el0ᴾ γ γᴾ x[γ] (xᴾ γ γᴾ)

El+maElimᴾ : (γ : Sub · Γ) (γᴾ : Γᴾ γ) →
        {j : MetaNat}(P : Tm Γ (Ma → (U j))
        → (el0 : Tm Γ (U0 → P $$ (El0' $$ q)))
        → (el+ : Tm Γ (Ma → P $$ q → (El $$ q¹ → Ma)
          → (lam (P[p] $$ (q¹ $$ q)))
          → U+ $$ (El $$ q³) $$ (lam (El[p] $$ (q² $$ q)))
          → P $$ (El+'  → (Aᴾ : Maᴾ A)$$ q⁴ $$ q² $$ q)))
          → (a : Tm ∙ Ma) → (b : Tm ∙ (El $$ A → Ma))
          → (x : Tm ∙ (U+ $$ (El $$ A) $$
                             (lam (El[p] $$ (B[p] $$ q)))))
  (maElim P el0 el+ (El+' a b x))ᴾ γ γᴾ
  ≡
  (el+ $$ a $$
    (maElim P el0 el+ a) $$ b $$
    (lam (maElim P[p] el0[p] el+[p] (b[p] $$ q)))
    $$ x)ᴾ γ γᴾ

  MaᴾElim P[γ] (Pᴾ γ γᴾ)
      el0[γ] (λ u uᴾ → el0ᴾ γ γᴾ u uᴾ) el+[γ]
      (λ A Aᴾ PA PAᴾ B Bᴾ PB PBᴾ C Cᴾ →
        el+ᴾ γ γᴾ A Aᴾ PA PAᴾ B Bᴾ PB PBᴾ C Cᴾ)
      (El+' a[γ] b[γ] x[γ])
      (El+'ᴾ a[γ] (aᴾ γ γᴾ)
        b[γ]
        (λ A Aᴾ → bᴾ γ γᴾ A Aᴾ) x[γ] (xᴾ γ γᴾ))
  ≡
  el+ᴾ γ γᴾ a[γ] (aᴾ γ γᴾ)
    (maElim P el0 el+ a)[γ]
    ((maElim P el0 el+ a)ᴾ γ γᴾ)
    b[γ] (λ A Aᴾ → bᴾ γ γᴾ A Aᴾ)
    (λ A → maElim P[γ] el0[γ] el+[γ] (b[γ] $$ A))
    (λ A Aᴾ → (maElim P el0 el+ (b $$ a))ᴾ γ γᴾ a aᵖ)
    x[γ] (x γ γᴾ)

  (λ A Aᴾ PA PAᴾ B Bᴾ PB PBᴾ C Cᴾ →
        el+ᴾ γ γᴾ A Aᴾ PA PAᴾ B Bᴾ PB PBᴾ C Cᴾ)
       a[γ] (aᴾ γ γᴾ) (maElim P[γ] el0[γ] el+[γ] a[γ])
      (MaᴾElim P[γ] (Pᴾ γ γᴾ) el0[γ] (λ u uᴾ → el0ᴾ γ γᴾ u uᴾ) el+[γ]
        (λ A Aᴾ PA PAᴾ B Bᴾ PB PBᴾ C Cᴾ →
          el+ᴾ γ γᴾ A Aᴾ PA PAᴾ B Bᴾ PB PBᴾ C Cᴾ) a[γ] (aᴾ γ γᴾ))
      b[γ] (λ A Aᴾ → bᴾ γ γᴾ A Aᴾ)
      (λ A → maElim P[γ] el0[γ] el+[γ] (B[γ] $$ A))
      (λ A Aᴾ →
      (MaᴾElim P[γ] (Pᴾ γ γᴾ) el0[γ] (λ u uᴾ → el0ᴾ γ γᴾ u uᴾ) el+[γ]
        (λ A Aᴾ PA PAᴾ B Bᴾ PB PBᴾ C Cᴾ →
          el+ᴾ γ γᴾ A Aᴾ PA PAᴾ B Bᴾ PB PBᴾ C Cᴾ)
          ((app b[γ]) $$ A) (bᴾ γ γᴾ A Aᴾ)))
      x[γ] (x γ γᴾ)
  ≡
  el+ᴾ γ γᴾ a[γ] (aᴾ γ γᴾ)
    (maElim P el0 el+ a)[γ]
    ((maElim P el0 el+ a)ᴾ γ γᴾ)
    b[γ] (λ A Aᴾ → bᴾ γ γᴾ A Aᴾ)
    (λ A → maElim P[γ] el0[γ] el+[γ] (b[γ] $$ A))
    (λ A Aᴾ → (maElim P el0 el+ (b $$ a))ᴾ γ γᴾ a aᵖ)
    x[γ] (x γ γᴾ)

  el+ᴾ γ γᴾ a[γ] (aᴾ γ γᴾ) (maElim P[γ] el0[γ] el+[γ] a[γ])
      (MaᴾElim P[γ] (Pᴾ γ γᴾ) el0[γ] (λ u uᴾ → el0ᴾ γ γᴾ u uᴾ) el+[γ]
        (λ A Aᴾ PA PAᴾ B Bᴾ PB PBᴾ C Cᴾ →
          el+ᴾ γ γᴾ A Aᴾ PA PAᴾ B Bᴾ PB PBᴾ C Cᴾ) a[γ] (aᴾ γ γᴾ))
      b[γ] (λ A Aᴾ → bᴾ γ γᴾ A Aᴾ)
      (λ A → maElim P[γ] el0[γ] el+[γ] (B[γ] $$ A))
      (λ A Aᴾ →
      (MaᴾElim P[γ] (Pᴾ γ γᴾ) el0[γ] (λ u uᴾ → el0ᴾ γ γᴾ u uᴾ) el+[γ]
        (λ A Aᴾ PA PAᴾ B Bᴾ PB PBᴾ C Cᴾ →
          el+ᴾ γ γᴾ A Aᴾ PA PAᴾ B Bᴾ PB PBᴾ C Cᴾ)
          ((app b[γ]) $$ A) (bᴾ γ γᴾ A Aᴾ)))
      x[γ] (x γ γᴾ)
  ≡
  el+ᴾ γ γᴾ a[γ] (aᴾ γ γᴾ) (maElim P[γ] el0[γ] el+[γ] a[γ])
      (MaᴾElim P[γ] (Pᴾ γ γᴾ) el0[γ] (λ u uᴾ → el0ᴾ γ γᴾ u uᴾ)
        el+[γ] (λ A Aᴾ PA PAᴾ B Bᴾ PB PBᴾ C Cᴾ →
                    el+ᴾ γ γᴾ A Aᴾ PA PAᴾ B Bᴾ PB PBᴾ C Cᴾ)
        a[γ] (aᴾ γ γᴾ))
      b[γ] (λ A Aᴾ → bᴾ γ γᴾ A Aᴾ)
      (λ A → maElim P[γ] el0[γ] el+[γ] (B[γ] $$ A))
      (λ A Aᴾ →
        (MaᴾElim P[γ] (Pᴾ γ γᴾ) el0[γ] (λ u uᴾ → el0ᴾ γ γᴾ u uᴾ)
        el+[γ] (λ A Aᴾ PA PAᴾ B Bᴾ PB PBᴾ C Cᴾ →
                  el+ᴾ γ γᴾ A Aᴾ PA PAᴾ B Bᴾ PB PBᴾ C Cᴾ)
          ((app b[γ]) $$ A) (bᴾ γ γᴾ A Aᴾ)))
      x[γ] (x γ γᴾ)


\end{verbatim}

\subsection{Substitution equations for the Mahlo canonicity model}

Proof that the predicates for Mahlo respect substitution.

\begin{verbatim}
subEl0ᴾ : (γ : Sub · Γ) (γᴾ : Γᴾ γ) → (δ : Sub Γ Δ)
                                    → (u : Tm Δ U0) →
 ((El0' u)[δ])ᴾ γ γᴾ
 ≡
 (El0' u[δ])ᴾ γ γᴾ

 (El0' u)ᴾ (δ ∘ γ) (δᴾ γ γᴾ)
 ≡
 (El0' u[δ])ᴾ γ γᴾ

 El0'ᴾ u[δ ∘ γ] (uᴾ (δ ∘ γ) (δᴾ γ γᴾ))
 ≡
 El0'ᴾ u[δ][γ] (u[δ]ᴾ γ γᴾ)

 El0'ᴾ u[δ ∘ γ] (uᴾ (δ ∘ γ) (δᴾ γ γᴾ))
 ≡
 El0'ᴾ u[δ ∘ γ] (uᴾ (δ ∘ γ) (δᴾ γ γᴾ))

subEl+ᴾ : (γ : Sub · Γ) (γᴾ : Γᴾ γ) → (δ : Sub Γ Δ)
        → (A : Tm Δ Ma)
        → (B : Tm Δ (El $$ A) → Ma)
        → (C : Tm ∙ (U+ $$ (El $$ A)
                        $$ (lam (El[p] $$ (B[p] $$ q))))) →
  ((El+' $$ A $$ B $$ C)[δ])ᴾ γ γᴾ
  ≡
  (El+' $$ A[δ] $$ B[δ] C[δ])ᴾ γ γᴾ

  (El+' $$ A $$ B $$ C)ᴾ (δ ∘ γ) (δᴾ γ γᴾ)
  ≡
  (El+' $$ A[δ] $$ B[δ] C[δ])ᴾ γ γᴾ

  El+'ᴾ A[δ ∘ γ] (Aᴾ (δ ∘ γ) (δᴾ γ γᴾ)) B[δ ∘ γ]
    (λ a aᴾ → (Bᴾ (δ ∘ γ) (δᴾ γ γᴾ) a aᴾ)
    C[δ ∘ γ] (Cᴾ (δ ∘ γ) (δᴾ γ γᴾ))
  ≡
  El+'ᴾ A[δ][γ] (A[δ]ᴾ γ γᴾ) B[δ][γ]
      (λ a aᴾ → (B[δ]ᴾ γ γᴾ a aᴾ) C[δ][γ] (C[δ]ᴾ γ γᴾ)

  El+'ᴾ A[δ ∘ γ] (Aᴾ (δ ∘ γ) (δᴾ γ γᴾ)) B[δ ∘ γ]
    (λ a aᴾ → (Bᴾ (δ ∘ γ) (δᴾ γ γᴾ) a aᴾ)
    C[δ ∘ γ] (Cᴾ (δ ∘ γ) (δᴾ γ γᴾ))
  ≡
  El+'ᴾ A[δ ∘ γ] (Aᴾ (δ ∘ γ) (δᴾ γ γᴾ)) B[δ ∘ γ]
      (λ a aᴾ → (Bᴾ (δ ∘ γ) (δᴾ γ γᴾ) a aᴾ) C[δ ∘ γ]
      (Cᴾ (δ ∘ γ) (δᴾ γ γᴾ))

submaElimᴾ : (γ : Sub · Γ) (γᴾ : Γᴾ γ) → (δ : Sub Γ Δ) →
        {j : MetaNat}(P : Tm Γ (Ma → (U j))
        → (el0 : Tm Γ (U0 → P $$ (El0' $$ q)))
        → (el+ : Tm Γ (Ma → P $$ q → (El $$ q¹ → Ma)
          → (lam (P[p] $$ (q¹ $$ q)))
          → U+ $$ (El $$ q³) $$ lam (El[p] $$ (q² $$ q))
          → P $$ (El+' $$ q⁴ $$ q² $$ q))) →
        (t : Tm Γ Ma) →
 ((maElim P el0 el+ t)[δ])ᴾ γ γᴾ
 ≡
 (maElim P[δ] el0[δ] el+[δ] t[δ])ᴾ γ γᵖ

 (maElim P el0 el+ t)ᴾ (δ ∘ γ) (δᴾ γ γᴾ)
 ≡
 (maElim P[δ] el0[δ] el+[δ] t[δ])ᴾ γ γᵖ

 MaᴾElim P[δ ∘ γ] (Pᴾ (δ ∘ γ) (δᴾ γ γᴾ))
        el0[δ ∘ γ] (λ u uᴾ → el0ᴾ (δ ∘ γ) (δᴾ γ γᴾ) u uᴾ)
        el+[δ ∘ γ] (λ A Aᴾ PA PAᴾ B Bᴾ PB PBᴾ C Cᴾ →
        el+ᴾ (δ ∘ γ) (δᴾ γ γᴾ) A Aᴾ PA PAᴾ B Bᴾ PB PBᴾ C Cᴾ)
        m[δ ∘ γ] (mᴾ (δ ∘ γ) (δᴾ γ γᴾ))
 ≡
 MaᴾElim P[δ][γ] ((P[δ])ᴾ γ γᴾ)
        el0[δ][γ] (λ u uᴾ → (el0[δ])ᴾ γ γᴾ u uᴾ)
        el+[δ][γ]
        (λ A Aᴾ PA PAᴾ B Bᴾ PB PBᴾ C Cᴾ →
        (el+[δ])ᴾ γ γᴾ A Aᴾ PA PAᴾ B Bᴾ PB PBᴾ C Cᴾ)
        m[δ][γ] ((m[δ])ᴾ γ γᴾ)

 MaᴾElim P[δ ∘ γ] (Pᴾ (δ ∘ γ) (δᴾ γ γᴾ))
        el0[δ ∘ γ] (λ u uᴾ → el0ᴾ (δ ∘ γ) (δᴾ γ γᴾ) u uᴾ)
        el+[δ ∘ γ] (λ A Aᴾ PA PAᴾ B Bᴾ PB PBᴾ C Cᴾ →
        el+ᴾ (δ ∘ γ) (δᴾ γ γᴾ) A Aᴾ PA PAᴾ B Bᴾ PB PBᴾ C Cᴾ)
        m[δ ∘ γ] (mᴾ (δ ∘ γ) (δᴾ γ γᴾ))
 ≡
 MaᴾElim P[δ ∘ γ] (Pᴾ (δ ∘ γ) (δᴾ γ γᴾ))
        el0[δ ∘ γ] (λ u uᴾ → el0ᴾ (δ ∘ γ) (δᴾ γ γᴾ) u uᴾ)
        el+[δ ∘ γ] (λ A Aᴾ PA PAᴾ B Bᴾ PB PBᴾ C Cᴾ →
        el+ᴾ (δ ∘ γ) (δᴾ γ γᴾ) A Aᴾ PA PAᴾ B Bᴾ PB PBᴾ C Cᴾ)
        m[δ ∘ γ] (mᴾ (δ ∘ γ) (δᴾ γ γᴾ))
\end{verbatim}
